refactor organisation of bootstrap theories
- move them all into subdirectories of bootstrap
- organise the subdirectories in three categories:
    translation, evaluation, and proofs
- move some other theorems around so that bootstrapping depends less
  on the compiler and repl correctness proofs (it still depends on
  compiler proofs for compute_free_varsLib - this can be fixed later)
- rename theories somewhat more consistently
- add/fix/update READMEs

(the main motivation was to put the compiler translation
 into a separate directory)

bootstrap/translation/repl/evaluateReplScript.sml
@@ -1,8 +1,8 @@
 open HolKernel boolLib bossLib lcsymtacs pairSyntax listTheory miscLib
 open ml_translatorTheory bigStepTheory terminationTheory
-open ml_repl_moduleTheory
+open replModuleTheory
 
-val _ = new_theory"evaluateReplDecs"
+val _ = new_theory"evaluateRepl"
 
 val () = Globals.max_print_depth := 20
 
@@ -21,7 +21,7 @@ val repl_all_env = ``^y,merge_alist_mod_env ^x (THE prim_sem_env).sem_envC,(THE 
 val repl_decs_cs =
   let
     val cs = listSimps.list_compset()
-    val _ = computeLib.add_thms[ml_repl_module_decls] cs
+    val _ = computeLib.add_thms[replModule_decls] cs
     val _ = computeLib.add_thms[rich_listTheory.LASTN_compute,
                                 evalPropsTheory.ctors_of_dec_def,
                                 evalPropsTheory.ctors_of_tdef_def] cs
@@ -31,10 +31,10 @@ val repl_decs_cs =
   end
 
 val last_3_decs = save_thm("last_3_decs",
-  computeLib.CBV_CONV repl_decs_cs ``LASTN 3 ml_repl_module_decls``)
+  computeLib.CBV_CONV repl_decs_cs ``LASTN 3 replModule_decls``)
 
 val append_3 = save_thm("append_3",
-  rich_listTheory.APPEND_BUTLASTN_LASTN |> Q.ISPECL[`3:num`,`ml_repl_module_decls`]
+  rich_listTheory.APPEND_BUTLASTN_LASTN |> Q.ISPECL[`3:num`,`replModule_decls`]
   |> UNDISCH |> SYM |> REWRITE_RULE[last_3_decs]
   |> prove_hyps_by(CONV_TAC(computeLib.CBV_CONV repl_decs_cs)))
 
@@ -48,22 +48,22 @@ val repl_env_def = new_specification("repl_env_def",["iloc","repl_env"],iloc_rep
 
 val sum_idx = ``21:num``
 val sym_idx = ``246:num``
-val el_sum = computeLib.CBV_CONV repl_decs_cs ``EL ^sum_idx ml_repl_module_decls``
-val take_sum = computeLib.CBV_CONV repl_decs_cs ``TAKE ^sum_idx ml_repl_module_decls``
-val drop_sum = computeLib.CBV_CONV repl_decs_cs ``DROP (^sum_idx + 1) ml_repl_module_decls``
-val el_sym = computeLib.CBV_CONV repl_decs_cs ``EL ^sym_idx ml_repl_module_decls``
-val take_sym = computeLib.CBV_CONV repl_decs_cs ``TAKE ^sym_idx ml_repl_module_decls``
-val drop_sym = computeLib.CBV_CONV repl_decs_cs ``DROP (^sym_idx + 1) ml_repl_module_decls``
-val length = save_thm("length_repl_decs",computeLib.CBV_CONV repl_decs_cs ``LENGTH ml_repl_module_decls``)
+val el_sum = computeLib.CBV_CONV repl_decs_cs ``EL ^sum_idx replModule_decls``
+val take_sum = computeLib.CBV_CONV repl_decs_cs ``TAKE ^sum_idx replModule_decls``
+val drop_sum = computeLib.CBV_CONV repl_decs_cs ``DROP (^sum_idx + 1) replModule_decls``
+val el_sym = computeLib.CBV_CONV repl_decs_cs ``EL ^sym_idx replModule_decls``
+val take_sym = computeLib.CBV_CONV repl_decs_cs ``TAKE ^sym_idx replModule_decls``
+val drop_sym = computeLib.CBV_CONV repl_decs_cs ``DROP (^sym_idx + 1) replModule_decls``
+val length = save_thm("length_repl_decs",computeLib.CBV_CONV repl_decs_cs ``LENGTH replModule_decls``)
 val tdefs_sum = prove(
-  ``ml_repl_module_decls = ^(lhs(concl take_sum)) ++ [^(lhs(concl el_sum))] ++ ^(lhs(concl drop_sum))``,
+  ``replModule_decls = ^(lhs(concl take_sum)) ++ [^(lhs(concl el_sum))] ++ ^(lhs(concl drop_sum))``,
   assume_tac length >>
   rw[LIST_EQ_REWRITE] >>
   Cases_on`x < ^sum_idx` >> simp[rich_listTheory.EL_APPEND1,rich_listTheory.EL_TAKE] >>
   Cases_on`x = ^sum_idx` >> simp[rich_listTheory.EL_APPEND1,rich_listTheory.EL_APPEND2] >>
   simp[rich_listTheory.EL_DROP])
 val tdefs_sym = prove(
-  ``ml_repl_module_decls = ^(lhs(concl take_sym)) ++ [^(lhs(concl el_sym))] ++ ^(lhs(concl drop_sym))``,
+  ``replModule_decls = ^(lhs(concl take_sym)) ++ [^(lhs(concl el_sym))] ++ ^(lhs(concl drop_sym))``,
   assume_tac length >>
   rw[LIST_EQ_REWRITE] >>
   Cases_on`x < ^sym_idx` >> simp[rich_listTheory.EL_APPEND1,rich_listTheory.EL_TAKE] >>
@@ -90,13 +90,13 @@ val sym_tags_exist = save_thm("sym_tags_exist",
 
 (* Define the compiler calls to bootstrap *)
 
-val compile_repl_decs_def = zDefine`
-  compile_repl_decs = compile_top NONE ((FST(THE prim_env)).comp_rs) (Tmod "REPL" NONE ml_repl_module_decls)`
+val compile_repl_module_def = zDefine`
+  compile_repl_module = compile_top NONE ((FST(THE prim_env)).comp_rs) (Tmod "REPL" NONE replModule_decls)`
 
 val call_dec = ``Tdec (Dlet (Plit Unit) (App Opapp [Var(Long"REPL""call_repl_step"); Lit Unit]))``
 
 val compile_call_repl_step_def = zDefine`
-  compile_call_repl_step = compile_special (FST compile_repl_decs) ^call_dec`
+  compile_call_repl_step = compile_special (FST compile_repl_module) ^call_dec`
 
 (* Effect of evaluating the call *)
 
@@ -152,7 +152,7 @@ val evaluate_call_repl_step = store_thm("evaluate_call_repl_step",
   qexists_tac`out'` >> simp[] >>
   simp[semanticPrimitivesTheory.store_lookup_def] >>
   simp[semanticPrimitivesTheory.store_assign_def] >>
-  Cases_on`Tmod_state"REPL"ml_repl_module_decls`>>
+  Cases_on`Tmod_state"REPL"replModule_decls`>>
   simp[update_io_def,PULL_EXISTS] >>
   qexists_tac`Litv Unit` >>
   simp[pmatch_def] >>
