bootstrap/evaluation/compileReplScript.sml
@@ -1,5 +1,5 @@
-open HolKernel boolLib bossLib evaluateReplDecsTheory flookupLib compute_compilerLib
-val _ = new_theory"compileReplDecs"
+open HolKernel boolLib bossLib evaluateReplTheory flookupLib compute_compilerLib
+val _ = new_theory"compileRepl"
 
 val _ = Globals.max_print_depth := 20
 
@@ -10,17 +10,17 @@ val () = computeLib.add_conv (finite_mapSyntax.flookup_t,2,FLOOKUP_DEFN_CONV) cs
 val () = computeLib.add_datatype_info cs (valOf(TypeBase.fetch``:comp_environment``))
 val eval = computeLib.CBV_CONV cs
 
-val compile_repl_decs_eq = save_thm("compile_repl_decs_eq",
-  time (REWR_CONV compile_repl_decs_def
-        THENC PURE_ONCE_REWRITE_CONV[ml_repl_moduleTheory.ml_repl_module_decls,initCompEnvTheory.prim_env_eq]
+val compile_repl_module_eq = save_thm("compile_repl_module_eq",
+  time (REWR_CONV compile_repl_module_def
+        THENC PURE_ONCE_REWRITE_CONV[replModuleTheory.replModule_decls,initCompEnvTheory.prim_env_eq]
         THENC eval)
-  ``compile_repl_decs``)
+  ``compile_repl_module``)
 
 val _ = computeLib.add_thms [compilerTheory.compile_special_def] cs
 val eval_special = computeLib.CBV_CONV cs
 val compile_call_repl_step_eq = save_thm("compile_call_repl_step_eq",
   time (REWR_CONV compile_call_repl_step_def THENC
-        PURE_ONCE_REWRITE_CONV[compile_repl_decs_eq] THENC
+        PURE_ONCE_REWRITE_CONV[compile_repl_module_eq] THENC
         eval_special)
   ``compile_call_repl_step``)
 
